\documentclass{article}

\usepackage[english]{babel}
\usepackage{mathtools}

\usepackage[letterpaper,top=2cm,bottom=2cm,left=3cm,right=3cm,marginparwidth=1.75cm]{geometry}

\title{Normalization}
\author{Ksenchik Nikita}

\begin{document}
\maketitle

Original expression:
$((\lambda a.(\lambda b.b\ b)\ (\lambda b.b\ b))\ b) ((\lambda c.(c\ b))\ (\lambda a.a))$

\begin{enumerate}
    \item $((\lambda a.(\lambda b.b\ b)\ (\lambda b.b\ b))\ b) ((\lambda c.(c\ b))\ (\lambda a.a))\ \rightarrow_\beta$
    \item $((\lambda b.b\ b)\ (\lambda b.b\ b))\ ((\lambda c.(c\ b))\ (\lambda a.a))\ \rightarrow_\beta$
    \item $((\lambda b.b\ b)\ (\lambda b.b\ b))\ ( (\lambda a.a)\ b)\ \rightarrow_\beta$
    \item $(\lambda b.b\ b)\ (\lambda b.b\ b)\ b$

\end{enumerate}

\end{document}
